Not bad

NoReacq.v
@@ -1,96 +1,315 @@
 From Elo Require Import Core.
 
 (* ------------------------------------------------------------------------- *)
+(* no-reacq                                                                  *)
+(* ------------------------------------------------------------------------- *)
+
+Inductive no_reacq (ad : addr) : tm -> Prop :=
+  | noreacq_unit  :                  no_reacq ad <{unit                     }>
+  | noreacq_nat   : forall n,        no_reacq ad <{nat n                    }>
+  | noreacq_plus  : forall t1 t2,    no_reacq ad t1 ->
+                                     no_reacq ad t2 ->
+                                     no_reacq ad <{t1 + t2                  }>
+  | noreacq_monus : forall t1 t2,    no_reacq ad t1 ->
+                                     no_reacq ad t2 ->
+                                     no_reacq ad <{t1 - t2                  }>
+  | noreacq_seq   : forall t1 t2,    no_reacq ad t1 ->
+                                     no_reacq ad t2 ->
+                                     no_reacq ad <{t1; t2                   }>
+  | noreacq_if    : forall t1 t2 t3, no_reacq ad t1 ->
+                                     no_reacq ad t2 ->
+                                     no_reacq ad t3 ->
+                                     no_reacq ad <{if t1 then t2 else t3 end}>
+  | noreacq_while : forall t1 t2,    no_reacq ad t1 ->
+                                     no_reacq ad t2 ->
+                                     no_reacq ad <{while t1 do t2 end       }>
+  | noreacq_var   : forall x,        no_reacq ad <{var x                    }>
+  | noreacq_fun   : forall x Tx t,   no_reacq ad t  ->
+                                     no_reacq ad <{fn x Tx t                }>
+  | noreacq_call  : forall t1 t2,    no_reacq ad t1 ->
+                                     no_reacq ad t2 ->
+                                     no_reacq ad <{call t1 t2               }>
+  | noreacq_ref   : forall ad' T,    no_reacq ad <{&ad' : T                 }>
+  | noreacq_new   : forall t T,      no_reacq ad t  ->
+                                     no_reacq ad <{new t : T                }>
+  | noreacq_init  : forall ad' t T,  no_reacq ad t  ->
+                                     no_reacq ad <{init ad' t : T           }>
+  | noreacq_load  : forall t,        no_reacq ad t  ->
+                                     no_reacq ad <{*t                       }>
+  | noreacq_asg   : forall t1 t2,    no_reacq ad t1 ->
+                                     no_reacq ad t2 ->
+                                     no_reacq ad <{t1 := t2                 }>
+  | noreacq_acq   : forall t1 x t2,  no_reacq ad t1 ->
+                                     no_reacq ad t2 ->
+                                     no_reacq ad <{acq t1 x t2              }>
+  | noreacq_cr    : forall ad' t,    no_reacq ad t  ->
+                                     no_reacq ad <{cr ad' t                 }>
+  | noreacq_wait  : forall t,        no_reacq ad t  ->
+                                     no_reacq ad <{wait t                   }>
+  | noreacq_reacq : forall ad',      ad <> ad'      ->
+                                     no_reacq ad <{reacq ad'                }>
+  | noreacq_spawn : forall t,        no_reacq ad t ->
+                                     no_reacq ad <{spawn t                  }>
+  .
+
+(* inversion --------------------------------------------------------------- *)
+
+Local Ltac _noreacq tt :=
+  match goal with
+  | H : no_reacq _   <{unit                  }> |- _ => clear H
+  | H : no_reacq _   <{nat _                 }> |- _ => clear H
+  | H : no_reacq _   <{_ + _                 }> |- _ => tt H
+  | H : no_reacq _   <{_ - _                 }> |- _ => tt H
+  | H : no_reacq _   <{_; _                  }> |- _ => tt H
+  | H : no_reacq _   <{if _ then _ else _ end}> |- _ => tt H
+  | H : no_reacq _   <{while _ do _ end      }> |- _ => tt H
+  | H : no_reacq _   <{var _                 }> |- _ => clear H
+  | H : no_reacq _   <{fn _ _ _              }> |- _ => tt H
+  | H : no_reacq _   <{call _ _              }> |- _ => tt H
+  | H : no_reacq _   <{&_ : _                }> |- _ => tt H
+  | H : no_reacq _   <{new _ : _             }> |- _ => tt H
+  | H : no_reacq _   <{init _ _ : _          }> |- _ => tt H
+  | H : no_reacq _   <{* _                   }> |- _ => tt H
+  | H : no_reacq _   <{_ := _                }> |- _ => tt H
+  | H : no_reacq _   <{acq _ _ _             }> |- _ => tt H
+  | H : no_reacq _   <{cr _ _                }> |- _ => tt H
+  | H : no_reacq _   <{wait _                }> |- _ => tt H
+  | H : no_reacq ?ad <{reacq ?ad             }> |- _ => invc H; auto
+  | H : no_reacq _   <{reacq _               }> |- _ => tt H
+  | H : no_reacq _   <{spawn _               }> |- _ => tt H
+  end.
+
+Ltac inv_noreacq  := _noreacq inv.
+Ltac invc_noreacq := _noreacq invc.
+
+(* lemmas ------------------------------------------------------------------ *)
+
+Lemma noreacq_wacq_contradiction : forall t1 t2 ad,
+  no_reacq ad t1 ->
+  t1 --[e_wacq ad]--> t2 ->
+  False.
+Proof.
+  intros. ind_tstep; invc_noreacq; auto.
+Qed.
+
+Lemma noreacq_wrel_contradiction : forall t1 t2 ad,
+  no_reacq ad t2 ->
+  t1 --[e_wrel ad]--> t2 ->
+  False.
+Proof.
+  intros. ind_tstep; invc_noreacq; auto.
+Qed.
+
+(* preservation lemmas ----------------------------------------------------- *)
+
+Lemma noreacq_subst : forall ad x tx t,
+  no_reacq ad t ->
+  no_reacq ad tx ->
+  no_reacq ad <{[x := tx] t}>.
+Proof.
+  intros. induction t; simpl; repeat destruct _str_eq_dec;
+  invc_noreacq; auto using no_reacq.
+Qed.
+
+(* preservation ------------------------------------------------------------ *)
+
+Local Ltac solve_noreacq_preservation :=
+  intros; ind_tstep; repeat invc_noreacq; auto using noreacq_subst, no_reacq.
+
+Lemma noreacq_preservation_none : forall ad t1 t2,
+  no_reacq ad t1 ->
+  t1 --[e_none]--> t2 ->
+  no_reacq ad t2.
+Proof. solve_noreacq_preservation. Qed.
+
+Lemma noreacq_preservation_alloc : forall ad t1 t2 ad' T',
+  no_reacq ad t1 ->
+  t1 --[e_alloc ad' T']--> t2 ->
+  no_reacq ad t2.
+Proof. solve_noreacq_preservation. Qed.
+
+Lemma noreacq_preservation_init : forall ad t1 t2 ad' t',
+  no_reacq ad t1 ->
+  t1 --[e_init ad' t']--> t2 ->
+  no_reacq ad t2.
+Proof. solve_noreacq_preservation. Qed.
+
+Lemma noreacq_preservation_read : forall ad t1 t2 ad' t',
+  no_reacq ad t' ->
+  (* --- *)
+  no_reacq ad t1 ->
+  t1 --[e_read ad' t']--> t2 ->
+  no_reacq ad t2.
+Proof. solve_noreacq_preservation. Qed.
+
+Lemma noreacq_preservation_write : forall ad t1 t2 ad' t',
+  no_reacq ad t1 ->
+  t1 --[e_write ad' t']--> t2 ->
+  no_reacq ad t2.
+Proof. solve_noreacq_preservation. Qed.
+
+Lemma noreacq_preservation_acq : forall ad t1 t2 ad' t',
+  no_reacq ad t' ->
+  (* --- *)
+  no_reacq ad t1 ->
+  t1 --[e_acq ad' t']--> t2 ->
+  no_reacq ad t2.
+Proof. solve_noreacq_preservation. Qed.
+
+Lemma noreacq_preservation_rel : forall ad t1 t2 ad',
+  no_reacq ad t1 ->
+  t1 --[e_rel ad']--> t2 ->
+  no_reacq ad t2.
+Proof. solve_noreacq_preservation. Qed.
+
+Lemma noreacq_preservation_wacq : forall ad t1 t2 ad',
+  no_reacq ad t1 ->
+  t1 --[e_wacq ad']--> t2 ->
+  no_reacq ad t2.
+Proof. solve_noreacq_preservation. Qed.
+
+Lemma noreacq_preservation_wrel : forall ad t1 t2 ad',
+  ad <> ad' ->
+  no_reacq ad t1 ->
+  t1 --[e_wrel ad']--> t2 ->
+  no_reacq ad t2.
+Proof. solve_noreacq_preservation. Qed.
+
+Lemma noreacq_preservation_spawn : forall ad t1 t2 t',
+  no_reacq ad t1 ->
+  t1 --[e_spawn t']--> t2 ->
+  no_reacq ad t2.
+Proof. solve_noreacq_preservation. Qed.
+
+Lemma noreacq_preservation_spawned : forall ad t1 t2 t',
+  no_reacq ad t1 ->
+  t1 --[e_spawn t']--> t2 ->
+  no_reacq ad t'.
+Proof. solve_noreacq_preservation. Qed.
+
+(* ------------------------------------------------------------------------- *)
 (* no-reacqs                                                                 *)
 (* ------------------------------------------------------------------------- *)
 
 (*
   (!!!) no-reacqs is an initial condition.
 *)
-Inductive no_reacqs : tm -> Prop :=
-  | noreacqs_unit  :                  no_reacqs <{unit                     }>
-  | noreacqs_nat   : forall n,        no_reacqs <{nat n                    }>
-  | noreacqs_plus  : forall t1 t2,    no_reacqs t1 ->
-                                      no_reacqs t2 ->
-                                      no_reacqs <{t1 + t2                  }>
-  | noreacqs_monus : forall t1 t2,    no_reacqs t1 ->
-                                      no_reacqs t2 ->
-                                      no_reacqs <{t1 - t2                  }>
-  | noreacqs_seq   : forall t1 t2,    no_reacqs t1 ->
-                                      no_reacqs t2 ->
-                                      no_reacqs <{t1; t2                   }>
-  | noreacqs_if    : forall t1 t2 t3, no_reacqs t1 ->
-                                      no_reacqs t2 ->
-                                      no_reacqs t3 ->
-                                      no_reacqs <{if t1 then t2 else t3 end}>
-  | noreacqs_while : forall t1 t2,    no_reacqs t1 ->
-                                      no_reacqs t2 ->
-                                      no_reacqs <{while t1 do t2 end       }>
-  | noreacqs_var   : forall x,        no_reacqs <{var x                    }>
-  | noreacqs_fun   : forall x Tx t,   no_reacqs t  ->
-                                      no_reacqs <{fn x Tx t                }>
-  | noreacqs_call  : forall t1 t2,    no_reacqs t1 ->
-                                      no_reacqs t2 ->
-                                      no_reacqs <{call t1 t2               }>
-  | noreacqs_ref   : forall ad T,     no_reacqs <{&ad : T                  }>
-  | noreacqs_new   : forall t T,      no_reacqs t  ->
-                                      no_reacqs <{new t : T                }>
-  | noreacqs_init  : forall ad t T,   no_reacqs t  ->
-                                      no_reacqs <{init ad t : T            }>
-  | noreacqs_load  : forall t,        no_reacqs t  ->
-                                      no_reacqs <{*t                       }>
-  | noreacqs_asg   : forall t1 t2,    no_reacqs t1 ->
-                                      no_reacqs t2 ->
-                                      no_reacqs <{t1 := t2                 }>
-  | noreacqs_acq   : forall t1 x t2,  no_reacqs t1 ->
-                                      no_reacqs t2 ->
-                                      no_reacqs <{acq t1 x t2              }>
-  | noreacqs_cr    : forall ad t,     no_reacqs t  ->
-                                      no_reacqs <{cr ad t                  }>
-  | noreacqs_wait  : forall t,        no_reacqs t  ->
-                                      no_reacqs <{wait t                   }>
-  | noreacqs_spawn : forall t,        no_reacqs t  ->
-                                      no_reacqs <{spawn t                  }>
-  .
+Definition no_reacqs (t : tm) := forall ad, no_reacq ad t.
 
 (* inversion --------------------------------------------------------------- *)
 
-Local Ltac _noreacqs tt :=
-  match goal with
-  | H : no_reacqs <{unit                  }> |- _ => clear H
-  | H : no_reacqs <{nat _                 }> |- _ => clear H
-  | H : no_reacqs <{_ + _                 }> |- _ => tt H
-  | H : no_reacqs <{_ - _                 }> |- _ => tt H
-  | H : no_reacqs <{_; _                  }> |- _ => tt H
-  | H : no_reacqs <{if _ then _ else _ end}> |- _ => tt H
-  | H : no_reacqs <{while _ do _ end      }> |- _ => tt H
-  | H : no_reacqs <{var _                 }> |- _ => clear H
-  | H : no_reacqs <{fn _ _ _              }> |- _ => tt H
-  | H : no_reacqs <{call _ _              }> |- _ => tt H
-  | H : no_reacqs <{&_ : _                }> |- _ => clear H
-  | H : no_reacqs <{new _ : _             }> |- _ => tt H
-  | H : no_reacqs <{init _ _ : _          }> |- _ => tt H
-  | H : no_reacqs <{* _                   }> |- _ => tt H
-  | H : no_reacqs <{_ := _                }> |- _ => tt H
-  | H : no_reacqs <{acq _ _ _             }> |- _ => tt H
-  | H : no_reacqs <{cr _ _                }> |- _ => tt H
-  | H : no_reacqs <{wait _                }> |- _ => tt H
-  | H : no_reacqs <{reacq _               }> |- _ => invc H
-  | H : no_reacqs <{spawn _               }> |- _ => tt H
-  end.
+Local Ltac solve_inv_noreacqs :=
+  unfold no_reacqs; intros; repeat split; intros; spec; invc_noreacq; auto.
 
-Ltac inv_noreacqs  := _noreacqs inv.
-Ltac invc_noreacqs := _noreacqs invc.
+Local Lemma inv_noreacqs_plus : forall t1 t2,
+  no_reacqs <{t1 + t2}> -> no_reacqs t1 /\ no_reacqs t2.
+Proof. solve_inv_noreacqs. Qed.
 
-(* decidability ------------------------------------------------------------ *)
+Local Lemma inv_noreacqs_monus : forall t1 t2,
+  no_reacqs <{t1 - t2}> -> no_reacqs t1 /\ no_reacqs t2.
+Proof. solve_inv_noreacqs. Qed.
 
-Lemma noreacqs_dec : forall t,
-  Decidable.decidable (no_reacqs t).
+Local Lemma inv_noreacqs_seq : forall t1 t2,
+  no_reacqs <{t1; t2}> -> no_reacqs t1 /\ no_reacqs t2.
+Proof. solve_inv_noreacqs. Qed.
+
+Local Lemma inv_noreacqs_if : forall t1 t2 t3,
+  no_reacqs (tm_if t1 t2 t3) -> no_reacqs t1 /\ no_reacqs t2 /\ no_reacqs t3.
+Proof. solve_inv_noreacqs. Qed.
+
+Local Lemma inv_noreacqs_while : forall t1 t2,
+  no_reacqs <{while t1 do t2 end}> -> no_reacqs t1 /\ no_reacqs t2.
+Proof. solve_inv_noreacqs. Qed.
+
+Local Lemma inv_noreacqs_fun : forall x Tx t,
+  no_reacqs <{fn x Tx t}> -> no_reacqs t.
+Proof. solve_inv_noreacqs. Qed.
+
+Local Lemma inv_noreacqs_call : forall t1 t2,
+  no_reacqs <{call t1 t2}> -> no_reacqs t1 /\ no_reacqs t2.
+Proof. solve_inv_noreacqs. Qed.
+
+Local Lemma inv_noreacqs_new : forall t T,
+  no_reacqs <{new t : T}> -> no_reacqs t.
+Proof. solve_inv_noreacqs. Qed.
+
+Local Lemma inv_noreacqs_init : forall ad t T,
+  no_reacqs <{init ad t : T}> -> no_reacqs t.
+Proof. solve_inv_noreacqs. Qed.
+
+Local Lemma inv_noreacqs_load : forall t,
+  no_reacqs <{*t}> -> no_reacqs t.
+Proof. solve_inv_noreacqs. Qed.
+
+Local Lemma inv_noreacqs_asg : forall t1 t2,
+  no_reacqs <{t1 := t2}> -> no_reacqs t1 /\ no_reacqs t2.
+Proof. solve_inv_noreacqs. Qed.
+
+Local Lemma inv_noreacqs_acq : forall t1 x t2,
+  no_reacqs <{acq t1 x t2}> -> no_reacqs t1 /\ no_reacqs t2.
+Proof. solve_inv_noreacqs. Qed.
+
+Local Lemma inv_noreacqs_cr : forall ad t,
+  no_reacqs <{cr ad t}> -> no_reacqs t.
+Proof. solve_inv_noreacqs. Qed.
+
+Local Lemma inv_noreacqs_wait : forall t,
+  no_reacqs <{wait t}> -> no_reacqs t.
+Proof. solve_inv_noreacqs. Qed.
+
+Local Lemma inv_noreacqs_reacq : forall ad,
+  no_reacqs <{reacq ad}> -> False.
+Proof. solve_inv_noreacqs. Qed.
+
+Local Lemma inv_noreacqs_spawn : forall t,
+  no_reacqs <{spawn t}> -> no_reacqs t.
+Proof. solve_inv_noreacqs. Qed.
+
+Ltac invc_noreacqs :=
+ match goal with
+ | H : no_reacqs <{unit        }> |- _ => clear H
+ | H : no_reacqs <{nat _       }> |- _ => clear H
+ | H : no_reacqs <{_ + _       }> |- _ => eapply inv_noreacqs_plus  in H
+ | H : no_reacqs <{_ - _       }> |- _ => eapply inv_noreacqs_monus in H
+ | H : no_reacqs <{_; _        }> |- _ => eapply inv_noreacqs_seq   in H
+ | H : no_reacqs (tm_if _ _ _  )  |- _ => eapply inv_noreacqs_if    in H
+ | H : no_reacqs (tm_while _ _ )  |- _ => eapply inv_noreacqs_while in H
+ | H : no_reacqs <{var _       }> |- _ => clear H
+ | H : no_reacqs <{fn _ _ _    }> |- _ => eapply inv_noreacqs_fun   in H
+ | H : no_reacqs <{call _ _    }> |- _ => eapply inv_noreacqs_call  in H
+ | H : no_reacqs <{& _ : _     }> |- _ => clear H
+ | H : no_reacqs <{new _ : _   }> |- _ => eapply inv_noreacqs_new   in H
+ | H : no_reacqs <{init _ _ : _}> |- _ => eapply inv_noreacqs_init  in H
+ | H : no_reacqs <{* _         }> |- _ => eapply inv_noreacqs_load  in H
+ | H : no_reacqs <{_ := _      }> |- _ => eapply inv_noreacqs_asg   in H
+ | H : no_reacqs <{acq _ _ _   }> |- _ => eapply inv_noreacqs_acq   in H
+ | H : no_reacqs <{cr _ _      }> |- _ => eapply inv_noreacqs_cr    in H
+ | H : no_reacqs <{wait _      }> |- _ => eapply inv_noreacqs_wait  in H
+ | H : no_reacqs <{reacq _     }> |- _ => eapply inv_noreacqs_reacq in H; auto
+ | H : no_reacqs <{spawn _     }> |- _ => eapply inv_noreacqs_spawn in H
+ end;
+ repeat match goal with
+ | H : no_reacqs _ /\ no_reacqs _                |- _ => destruct H
+ | H : no_reacqs _ /\ no_reacqs _ /\ no_reacqs _ |- _ => destruct H as [? [? ?]]
+ end.
+
+(* lemmas ------------------------------------------------------------------ *)
+
+Corollary noreacq_from_noreacqs : forall ad t,
+  no_reacqs t ->
+  no_reacq ad t.
 Proof.
-  unfold Decidable.decidable. unfold not. intros.
-  induction t; auto using no_reacqs;
-  try (destruct IHt1, IHt2, IHt3 || destruct IHt1, IHt2 || destruct IHt);
-  auto using no_reacqs;
-  right; intros; invc_noreacqs; auto.
+  unfold no_reacqs. trivial.
 Qed.
+
+(* preservation lemmas ----------------------------------------------------- *)
+
+Corollary noreacqs_subst : forall x tx t,
+  no_reacqs t ->
+  no_reacqs tx ->
+  no_reacqs <{[x := tx] t}>.
+Proof.
+  intros ** ?. auto using noreacq_subst.
+Qed.
+
 
