UniqueCRs.v
@@ -1,22 +1,107 @@
 From Elo Require Import Core.
 
 From Elo Require Import NoCR.
+From Elo Require Import NoReacq.
 From Elo Require Import ValidTerm.
 From Elo Require Import OneCR.
+From Elo Require Import IsWaiting.
+From Elo Require Import InCR.
+
+(* TODO: move *)
+From Elo Require Import ConsistentWaits.
+
+Local Lemma noreacq_from_nocr' : forall ad t wr,
+  wr <> WR_ad ad        ->
+  consistent_waits wr t ->
+  (* --- *)
+  no_cr    ad t ->
+  no_reacq ad t.
+Proof.
+  intros ? ?. induction t; intros; invc_cw; invc_nocr; eauto using no_reacq;
+  constructor; eauto;
+  match goal with
+  | IH : forall _, _ <> _ -> consistent_waits _ ?t -> _ -> no_reacq _ ?t
+  , H  : consistent_waits ?wr ?t
+  |- no_reacq _ ?t =>
+      eapply (IH wr); eauto
+  end;
+  intros F; invc F. auto.
+Qed.
+
+Corollary noreacq_from_nocr : forall ad t,
+  consistent_waits WR_none t ->
+  (* --- *)
+  no_cr    ad t ->
+  no_reacq ad t.
+Proof.
+  intros. eapply noreacq_from_nocr'; eauto. intros F. invc F.
+Qed.
+
+Local Lemma nocr_wacq_contradiction' : forall ad t1 t2 wr,
+  wr <> WR_ad ad         ->
+  consistent_waits wr t1 ->
+  (* --- *)
+  no_cr ad t1            ->
+  t1 --[e_wacq ad]--> t2 ->
+  False.
+Proof.
+  intros. gendep wr. ind_tstep; intros; invc_cw; invc_nocr; eauto.
+  spec. spec.
+  match goal with IH : _ -> _ -> _ -> False, H : consistent_waits ?wr _ |- _ =>
+   eapply (IH wr); eauto
+  end.
+  intros F. invc F. auto.
+Qed.
+
+Corollary nocr_wacq_contradiction : forall ad t1 t2,
+  consistent_waits WR_none t1 ->
+  (* --- *)
+  no_cr ad t1            ->
+  t1 --[e_wacq ad]--> t2 ->
+  False.
+Proof.
+  intros. eapply nocr_wacq_contradiction'; eauto. intros F. invc F.
+Qed.
+
+Local Lemma nocr_wrel_contradiction' : forall ad t1 t2 wr,
+  wr <> WR_ad ad         ->
+  consistent_waits wr t1 ->
+  (* --- *)
+  no_cr ad t1            ->
+  t1 --[e_wrel ad]--> t2 ->
+  False.
+Proof.
+  intros. gendep wr. ind_tstep; intros; invc_cw; invc_nocr; eauto.
+  spec. spec.
+  match goal with IH : _ -> _ -> _ -> False, H : consistent_waits ?wr _ |- _ =>
+   eapply (IH wr); eauto
+  end.
+  intros F. invc F. auto.
+Qed.
+
+Corollary nocr_wrel_contradiction : forall ad t1 t2,
+  consistent_waits WR_none t1 ->
+  (* --- *)
+  no_cr ad t1            ->
+  t1 --[e_wrel ad]--> t2 ->
+  False.
+Proof.
+  intros. eapply nocr_wrel_contradiction'; eauto. intros F. invc F.
+Qed.
 
 (* ------------------------------------------------------------------------- *)
 (* unique-critical-regions                                                   *)
 (* ------------------------------------------------------------------------- *)
 
 Definition unique_critical_regions (m : mem) (ths : threads) := forall ad,
-  (m[ad].X = false -> forall_threads ths (no_cr ad)) /\
-  (m[ad].X = true  -> forone_thread  ths (one_cr ad) (no_cr ad)).
+  (m[ad].X = false -> forall_threads ths (not_in_cr ad)) /\
+  (m[ad].X = true  -> forone_thread  ths (in_cr ad) (not_in_cr ad)).
 
 (* lemmas ------------------------------------------------------------------ *)
 
-Corollary nocr_or_onecr_from_ucr : forall ad m ths tid,
+Corollary incr_or_nincr_from_ucr : forall ad m ths tid,
   unique_critical_regions m ths ->
-  no_cr ad ths[tid] \/ one_cr ad ths[tid].
+  in_cr ad ths[tid] \/ not_in_cr ad ths[tid].
 Proof.
   intros * Hucr. specialize (Hucr ad) as [? Htrue].
   destruct (m[ad].X); spec; eauto.
@@ -24,55 +109,72 @@ Proof.
   nat_eq_dec tid' tid; auto.
 Qed.
 
-Corollary ucr_onecr_contradiction : forall ad m ths tid1 tid2,
+Corollary ucr_incr_contradiction : forall ad m ths tid1 tid2,
   unique_critical_regions m ths ->
   (* --- *)
   tid1 <> tid2 ->
-  one_cr ad ths[tid1] ->
-  one_cr ad ths[tid2] ->
+  in_cr ad ths[tid1] ->
+  in_cr ad ths[tid2] ->
   False.
 Proof.
   intros * Hucr **. specialize (Hucr ad) as [? Htrue].
   destruct (m[ad].X); spec;
-  eauto using nocr_onecr_contradiction.
+  eauto using nincr_incr_contradiction.
   specialize Htrue as [tid [? ?]].
   nat_eq_dec tid1 tid; nat_eq_dec tid2 tid;
-  eauto using nocr_onecr_contradiction.
+  eauto using nincr_incr_contradiction.
 Qed.
 
-Corollary ucr_onecr_equality : forall ad m ths tid1 tid2,
+Corollary ucr_incr_equality : forall ad m ths tid1 tid2,
   unique_critical_regions m ths ->
   (* --- *)
-  one_cr ad ths[tid1] ->
-  one_cr ad ths[tid2] ->
+  in_cr ad ths[tid1] ->
+  in_cr ad ths[tid2] ->
   tid1 = tid2.
 Proof.
   intros. nat_eq_dec tid1 tid2; trivial. exfalso.
-  eauto using ucr_onecr_contradiction.
+  eauto using ucr_incr_contradiction.
 Qed.
 
-Lemma locked_from_onecr : forall m ths tid ad,
+Lemma locked_from_incr : forall m ths tid ad,
   unique_critical_regions m ths ->
   (* --- *)
-  one_cr ad ths[tid] ->
+  in_cr ad ths[tid] ->
   m[ad].X = true.
 Proof.
   intros * Hucr ?.
   destruct (m[ad].X) eqn:Heq; trivial.
   specialize (Hucr ad) as [? _]. spec.
-  exfalso. eauto using nocr_onecr_contradiction.
+  exfalso. eauto using nincr_incr_contradiction.
 Qed.
 
 Lemma locked_from_rel : forall m ths tid t ad,
-  unique_critical_regions m ths ->
+  forall_threads ths (valid_term m) ->
+  unique_critical_regions m ths     ->
   (* --- *)
   ths[tid] --[e_rel ad]--> t ->
   m[ad].X = true.
 Proof.
-  intros * Hucr ?.
+  intros * ? Hucr ?.
   destruct (m[ad].X) eqn:Heq; trivial.
-  specialize (Hucr ad) as [? _]. spec.
-  exfalso. eauto using nocr_rel_contradiction.
+  specialize (Hucr ad) as [Hnincr _]. spec.
+  exfalso. specialize (Hnincr tid) as [? | ?];
+  eauto using nocr_rel_contradiction, isw_effect_contradiction.
+Qed.
+
+Lemma locked_from_wrel : forall m ths tid t ad,
+  forall_threads ths (valid_term m) ->
+  forall_threads ths (consistent_waits WR_none) ->
+  unique_critical_regions m ths     ->
+  (* --- *)
+  ths[tid] --[e_wrel ad]--> t ->
+  m[ad].X = true.
+Proof.
+  intros * ? ? Hucr ?.
+  destruct (m[ad].X) eqn:Heq; trivial.
+  specialize (Hucr ad) as [Hnincr _]. spec.
+  exfalso. specialize (Hnincr tid) as [? | ?];
+  eauto using nocr_wrel_contradiction, isw_effect_contradiction.
 Qed.
 
 (* preservation lemmas ----------------------------------------------------- *)
@@ -99,58 +201,61 @@ Proof.
   intros until 1.
   intros ? Hucr ? ad. specialize (Hucr ad) as [Hfall Hfone].
   split; intros; spec.
-  - intros ?. omicron; eauto using nocr_preservation_none.
+  - intros ?. omicron; eauto using nincr_preservation_none.
   - specialize Hfone as [tid' [? ?]]. exists tid'. split; intros; omicron;
-    eauto using nocr_preservation_none, onecr_preservation_none.
+    eauto using nincr_preservation_none, incr_preservation_none.
 Qed.
 
-Local Lemma ucr_preservation_alloc : forall m ths tid t T,
+Local Lemma ucr_preservation_alloc : forall m ths tid t T R,
   tid < #ths ->
   unique_critical_regions m ths ->
   ths[tid] --[e_alloc (#m) T]--> t ->
-  unique_critical_regions (m +++ new_cell T) ths[tid <- t].
+  unique_critical_regions (m +++ new_cell T R) ths[tid <- t].
 Proof.
   intros *.
   intros ? Hucr ? ad. specialize (Hucr ad) as [Hfall Hfone].
   split; intros; upsilon; spec.
-  - intros ?. omicron; eauto using nocr_preservation_alloc.
+  - intros ?. omicron; eauto using nincr_preservation_alloc.
   - specialize Hfone as [tid' [? ?]]. exists tid'.
     split; intros; omicron;
-    eauto using nocr_preservation_alloc, onecr_preservation_alloc.
+    eauto using nincr_preservation_alloc, incr_preservation_alloc.
 Qed.
 
-Local Lemma ucr_preservation_insert : forall m ths tid t ad' t',
+Local Lemma ucr_preservation_init : forall m ths tid t ad' t',
   forall_threads ths (valid_term m) ->
   (* --- *)
   tid < #ths ->
   unique_critical_regions m ths ->
-  ths[tid] --[e_insert ad' t']--> t ->
+  ths[tid] --[e_init ad' t']--> t ->
   unique_critical_regions m[ad'.t <- t'] ths[tid <- t].
 Proof.
   intros until 1.
   intros ? Hucr ? ad. specialize (Hucr ad) as [Hfall Hfone].
-  assert (ad' < #m) by eauto using vtm_insert_address.
-  split; intros; repeat omicron; spec; upsilon;
-  eauto using nocr_preservation_insert;
-  specialize Hfone as [tid' [? ?]]; exists tid'; split; intros;
-  omicron; eauto using nocr_preservation_insert, onecr_preservation_insert.
+  assert (ad' < #m) by eauto using vtm_init_address.
+  split; intros; omicron; upsilon; spec; solve
+    [ intro; omicron; eauto using nincr_preservation_init
+    | specialize Hfone as [tid' [? ?]]; exists tid';
+      split; intros; omicron;
+      eauto using nincr_preservation_init, incr_preservation_init
+    ].
 Qed.
 
 Local Lemma ucr_preservation_read : forall m ths tid t ad te,
-  no_crs te ->
+  value te ->
+  valid_term m te ->
   (* --- *)
   tid < #ths ->
   unique_critical_regions m ths ->
   ths[tid] --[e_read ad te]--> t ->
   unique_critical_regions m ths[tid <- t].
 Proof.
-  intros until 1.
+  intros until 2.
   intros ? Hucr ? ad'. specialize (Hucr ad') as [Hfall Hfone].
   split; intros; upsilon; spec.
-  - intros ?. omicron; eauto using nocr_preservation_read.
+  - intros ?. omicron; eauto using nincr_preservation_read.
   - specialize Hfone as [tid' [? ?]]. exists tid'.
     split; intros; omicron;
-    eauto using nocr_preservation_read, onecr_preservation_read.
+    eauto using nincr_preservation_read, incr_preservation_read.
 Qed.
 
 Local Lemma ucr_preservation_write : forall m ths tid t ad te,
@@ -165,110 +270,175 @@ Proof.
   intros ? Hucr ? ad'. specialize (Hucr ad') as [Hfall Hfone].
   assert (ad < #m) by eauto using vtm_write_address.
   split; intros; repeat omicron; spec; upsilon;
-  eauto using nocr_preservation_write;
+  eauto using nincr_unit, nincr_preservation_write;
   specialize Hfone as [tid' [? ?]]; exists tid'; split; intros;
-  omicron; eauto using nocr_preservation_write, onecr_preservation_write.
+  omicron; eauto using nincr_preservation_write, incr_preservation_write.
 Qed.
 
 Local Lemma ucr_preservation_acq : forall m ths tid ad t te,
-  no_crs te ->
+  value te ->
+  valid_term m te ->
+  forall_threads ths (valid_term m) ->
+  forall_threads ths (consistent_waits WR_none) ->
   (* --- *)
-  ad < #m ->
   m[ad].X = false ->
   tid < #ths ->
   unique_critical_regions m ths ->
   ths[tid] --[e_acq ad te]--> t ->
   unique_critical_regions m[ad.X <- true] ths[tid <- t].
 Proof.
-  intros until 3.
+  intros until 5.
   intros ? Hucr ? ad'. specialize (Hucr ad') as [Hfall Hfone].
+  assert (ad < #m) by eauto using vtm_acq_address.
   split; intros; repeat omicron; spec; upsilon;
-  eauto using nocr_preservation_acq.
+  eauto using nincr_unit, nincr_preservation_acq.
   - exists tid. sigma. split.
-    + eauto using nocr_to_onecr.
+    + split.
+      * specialize (Hfall tid) as [? | ?].
+        ** eauto using nocrs_from_value, nocr_to_onecr.
+        ** exfalso. eauto using isw_effect_contradiction.
+      * specialize (Hfall tid) as [? | ?].
+        ** eauto using noreacq_from_value, noreacq_preservation_acq,
+            noreacq_from_nocr.
+        ** exfalso. eauto using isw_effect_contradiction.
     + intros. sigma. eauto.
   - specialize Hfone as [tid' [? ?]]. exists tid'. split.
-    + omicron; eauto using onecr_preservation_acq.
-    + intros. omicron; eauto using nocr_preservation_acq.
+    + omicron; eauto using incr_preservation_acq.
+    + intros. omicron; eauto using nincr_preservation_acq.
 Qed.
 
 Local Lemma ucr_preservation_rel : forall m ths tid ad t,
+  forall_threads ths (valid_term m) ->
+  (* --- *)
   tid < #ths ->
   unique_critical_regions m ths ->
   ths[tid] --[e_rel ad]--> t ->
   unique_critical_regions m[ad.X <- false] ths[tid <- t].
 Proof.
-  intros *.
+  intros until 1.
   intros ? Hucr ? ad'. destruct (Hucr ad') as [Hfall Hfone].
   assert (Had : m[ad].X = true) by eauto using locked_from_rel.
   split; intros; try intros tid'; repeat omicron; spec; upsilon;
-  eauto using nocr_preservation_rel;
-  specialize Hfone as [tid'' [? ?]].
-  - nat_eq_dec tid'' tid'; eauto using onecr_to_nocr.
-    exfalso. eauto using nocr_rel_contradiction.
-  - nat_eq_dec tid'' tid'; eauto using nocr_rel_contradiction.
+  auto; eauto using nincr_preservation_rel;
+  specialize Hfone as [tid'' [Hincr Hnincr]].
+  - destruct Hincr. nat_eq_dec tid'' tid'.
+    + left. eauto using onecr_to_nocr.
+    + specialize (Hnincr tid'). spec. destruct Hnincr; exfalso;
+      eauto using nocr_rel_contradiction, isw_effect_contradiction.
+  - nat_eq_dec tid'' tid'; auto.
+    specialize (Hnincr tid). spec. destruct Hnincr; exfalso;
+    eauto using nocr_rel_contradiction, isw_effect_contradiction.
   - exists tid''. nat_eq_dec tid'' tid; sigma;
-    split; eauto using onecr_preservation_rel; intros.
+    split; eauto using incr_preservation_rel; intros.
     + sigma. auto.
-    + omicron; eauto using nocr_preservation_rel.
+    + omicron; eauto using nincr_preservation_rel.
+Qed.
+
+Local Lemma ucr_preservation_wacq : forall m ths tid t ad,
+  forall_threads ths (valid_term m) ->
+  forall_threads ths (consistent_waits WR_none) ->
+  (* --- *)
+  ad < #m ->
+  m[ad].X = false ->
+  tid < #ths ->
+  unique_critical_regions m ths ->
+  ths[tid] --[e_wacq ad]--> t ->
+  unique_critical_regions m[ad.X <- true] ths[tid <- t].
+Proof.
+  intros until 4.
+  intros ? Hucr ? ad'. specialize (Hucr ad') as [Hfall Hfone].
+  split; intros; repeat omicron; spec; upsilon;
+  eauto using nincr_unit, nincr_preservation_wacq.
+  - exists tid. sigma. split.
+    + split.
+      * specialize (Hfall tid) as [? | ?].
+        ** exfalso. eauto using noreacq_from_nocr, noreacq_wacq_contradiction.
+        ** admit. (* onecr_from_isw *)
+      * specialize (Hfall tid) as [? | ?].
+        ** eauto using nocr_preservation_wacq, cw_preservation_wacq,
+            noreacq_from_nocr.
+        ** eauto using isw_to_noreacq.
+    + intros. sigma. eauto.
+  - specialize Hfone as [tid' [? ?]]. exists tid'. split.
+    + omicron; eauto using incr_preservation_wacq.
+    + intros. omicron; eauto using nincr_preservation_wacq.
+Abort.
+
+Local Lemma ucr_preservation_wrel : forall m ths tid ad t,
+  forall_threads ths (valid_term m) ->
+  forall_threads ths (consistent_waits WR_none) ->
+  (* --- *)
+  tid < #ths ->
+  unique_critical_regions m ths ->
+  ths[tid] --[e_wrel ad]--> t ->
+  unique_critical_regions m[ad.X <- false] ths[tid <- t].
+Proof.
+  intros until 2.
+  intros ? Hucr ? ad'. destruct (Hucr ad') as [Hfall Hfone].
+  assert (Had : m[ad].X = true) by eauto using locked_from_wrel.
+  split; intros; try intros tid'; repeat omicron; spec; upsilon;
+  auto; eauto using nincr_preservation_wrel;
+  specialize Hfone as [tid'' [Hincr Hnincr]].
+  - destruct Hincr. nat_eq_dec tid'' tid'.
+    + right. eauto using noreacq_to_isw.
+    + specialize (Hnincr tid'). spec. exfalso. destruct Hnincr.
+      * eauto using nocr_wrel_contradiction.
+      * eauto using isw_effect_contradiction.
+  - nat_eq_dec tid'' tid'; auto.
+    destruct Hincr. specialize (Hnincr tid). spec. exfalso. destruct Hnincr.
+    + eauto using nocr_wrel_contradiction.
+    + eauto using isw_effect_contradiction.
+  - exists tid''. nat_eq_dec tid'' tid; sigma;
+    split; eauto using incr_preservation_wrel; intros.
+    + sigma. auto.
+    + omicron; eauto using nincr_preservation_wrel.
 Qed.
 
 Local Ltac eapply_in_tstep tt :=
   match goal with Htstep : _ --[_]--> _ |- _ => eapply tt in Htstep as ? end.
 
-Local Lemma ucr_preservation_spawn : forall m ths tid t te,
+Local Lemma ucr_preservation_spawn : forall m ths tid t t',
   forall_threads ths (valid_term m) ->
   (* --- *)
   tid < #ths ->
   unique_critical_regions m ths ->
-  ths[tid] --[e_spawn (#ths) te]--> t ->
-  unique_critical_regions m (ths[tid <- t] +++ te).
+  ths[tid] --[e_spawn t']--> t ->
+  unique_critical_regions m (ths[tid <- t] +++ t').
 Proof.
   intros until 1.
   intros ? Hucr ? ad'. destruct (Hucr ad') as [Hfall Hfone].
-  split; intros; repeat omicron; spec; upsilon.
-  - eapply_in_tstep nocr_preservation_spawn; eauto using no_cr.
-  - eauto using nocr_preservation_spawned.
-  - specialize Hfone as [tid' [? ?]]. exists tid'. omicron;
-    try invc_onecr; split; eauto using onecr_preservation_spawn; intros;
-    omicron; eauto using no_cr.
-    + eapply_in_tstep nocrs_spawn_term; eauto.
-    + eauto using nocr_preservation_spawn.
-    + eapply_in_tstep nocrs_spawn_term; eauto.
+  split; intros; spec.
+  - intro. omicron;
+    eauto using nincr_preservation_spawn, nincr_unit.
+    left. eauto using nocr_spawn_term.
+  - specialize Hfone as [tid' [Hincr Hnincr]]. exists tid'. split.
+    + omicron; eauto.
+      * eauto using incr_preservation_spawn.
+      * destruct Hincr. invc_onecr.
+    + intros. omicron; eauto using nincr_preservation_spawn, nincr_unit.
+      left. eauto using nocr_spawn_term.
 Qed.
 
 Theorem ucr_preservation_cstep : forall m1 m2 ths1 ths2 tid e,
   forall_memory  m1 value                ->
   forall_program m1 ths1 (valid_term m1) ->
+  forall_program m1 ths1 (consistent_waits WR_none) ->
   (* --- *)
   unique_critical_regions m1 ths1 ->
   m1 \ ths1 ~~[tid, e]~~> m2 \ ths2 ->
   unique_critical_regions m2 ths2.
 Proof.
-  intros * ? [? ?] **. invc_cstep; try invc_mstep.
+  intros * ? [? ?] [? ?] **. invc_cstep; try invc_mstep.
   - eauto using ucr_preservation_none.
-  - eauto using ucr_preservation_alloc.
-  - eauto using ucr_preservation_insert.
-  - eauto using nocrs_from_value, ucr_preservation_read.
+  - sigma. upsilon. eauto using ucr_preservation_alloc.
+  - eauto using ucr_preservation_init.
+  - eauto using ucr_preservation_read.
   - eauto using ucr_preservation_write.
-  - eauto using nocrs_from_value, ucr_preservation_acq.
+  - eauto using ucr_preservation_acq.
   - eauto using ucr_preservation_rel.
+  - admit. (* eauto using ucr_preservation_wacq. *)
+  - eauto using ucr_preservation_wrel.
   - eauto using ucr_preservation_spawn.
-Qed.
-
-Theorem ucr_preservation_rstep : forall m1 m2 ths1 ths2 tid e,
-  forall_memory  m1 value                ->
-  forall_program m1 ths1 (valid_term m1) ->
-  (* --- *)
-  unique_critical_regions m1 ths1 ->
-  m1 \ ths1 ~~~[tid, e]~~> m2 \ ths2 ->
-  unique_critical_regions m2 ths2.
-Proof.
-  intros. invc_rstep; eauto using ucr_preservation_cstep.
-  match goal with _ : _ \ _ ~~[_, _]~~> ?m \ ?ths |- _ =>
-    assert (unique_critical_regions m ths)
-  end;
-  eauto using ucr_preservation_cstep, ucr_mem_region.
 Qed.
 
 Theorem ucr_preservation_base : forall t,
@@ -277,7 +447,7 @@ Theorem ucr_preservation_base : forall t,
   unique_critical_regions nil (base t).
 Proof.
   unfold base. intros ** ?. split; intros Hnil.
-  - intro. omicron; auto using no_cr.
+  - intro. left. omicron; auto using no_cr.
   - simpl in Hnil. destruct ad; upsilon; auto.
 Qed.
 
