InCR.v
@@ -1,0 +1,290 @@
+From Elo Require Import Core.
+
+From Elo Require Import NoCR.
+From Elo Require Import NoReacq.
+From Elo Require Import ValidTerm.
+From Elo Require Import OneCR.
+From Elo Require Import IsWaiting.
+
+(* ------------------------------------------------------------------------- *)
+(* in-cr & not-in-cr                                                         *)
+(* ------------------------------------------------------------------------- *)
+
+Definition in_cr (ad : addr) (t : tm) := one_cr ad t /\ no_reacq ad t.
+
+Definition not_in_cr (ad : addr) (t : tm) := no_cr ad t \/ is_waiting ad t.
+
+(* lemmas ------------------------------------------------------------------ *)
+
+Corollary nincr_unit : forall ad,
+  not_in_cr ad <{unit}>.
+Proof.
+  intros. left. auto using no_cr.
+Qed.
+
+Corollary nincr_from_value : forall m ad t,
+  valid_term m t ->
+  (* --- *)
+  value t ->
+  not_in_cr ad t.
+Proof.
+  intros. left. eauto using nocr_from_value.
+Qed.
+
+Corollary nincr_incr_contradiction : forall ad t,
+  not_in_cr ad t ->
+  in_cr     ad t ->
+  False.
+Proof.
+  intros * [? | ?] [? ?];
+  eauto using nocr_onecr_contradiction, noreacq_isw_contradiction.
+Qed.
+
+(* preservation (incr) ----------------------------------------------------- *)
+
+Local Ltac solve_incr_preservation L1 L2 :=
+  intros; match goal with H : in_cr _ _ |- _ => destruct H end; split;
+  eauto using nocr_from_value, noreacq_from_value, L1, L2.
+
+Corollary incr_preservation_none : forall ad m t1 t2,
+  valid_term m t1 ->
+  (* --- *)
+  in_cr ad t1 ->
+  t1 --[e_none]--> t2 ->
+  in_cr ad t2.
+Proof.
+  solve_incr_preservation
+    onecr_preservation_none
+    noreacq_preservation_none.
+Qed.
+
+Corollary incr_preservation_alloc : forall ad t1 t2 ad' T',
+  in_cr ad t1 ->
+  t1 --[e_alloc ad' T']--> t2 ->
+  in_cr ad t2.
+Proof.
+  solve_incr_preservation
+    onecr_preservation_alloc
+    noreacq_preservation_alloc.
+Qed.
+
+Corollary incr_preservation_init : forall ad m t1 t2 ad' t',
+  valid_term m t1 ->
+  (* --- *)
+  in_cr ad t1 ->
+  t1 --[e_init ad' t']--> t2 ->
+  in_cr ad t2.
+Proof.
+  solve_incr_preservation
+    onecr_preservation_init
+    noreacq_preservation_init.
+Qed.
+
+Corollary incr_preservation_read : forall ad m t1 t2 ad' t',
+  valid_term m t' ->
+  value t'        ->
+  (* --- *)
+  in_cr ad t1 ->
+  t1 --[e_read ad' t']--> t2 ->
+  in_cr ad t2.
+Proof.
+  solve_incr_preservation
+    onecr_preservation_read
+    noreacq_preservation_read.
+Qed.
+
+Corollary incr_preservation_write : forall ad m t1 t2 ad' t',
+  valid_term m t1 ->
+  (* --- *)
+  in_cr ad t1 ->
+  t1 --[e_write ad' t']--> t2 ->
+  in_cr ad t2.
+Proof.
+  solve_incr_preservation
+    onecr_preservation_write
+    noreacq_preservation_write.
+Qed.
+
+Corollary incr_preservation_acq : forall ad m t1 t2 ad' t',
+  valid_term m t' ->
+  value t'        ->
+  (* --- *)
+  ad <> ad' ->
+  in_cr ad t1 ->
+  t1 --[e_acq ad' t']--> t2 ->
+  in_cr ad t2.
+Proof.
+  solve_incr_preservation
+    onecr_preservation_acq
+    noreacq_preservation_acq.
+Qed.
+
+Corollary incr_preservation_rel : forall ad t1 t2 ad',
+  ad <> ad' ->
+  in_cr ad t1 ->
+  t1 --[e_rel ad']--> t2 ->
+  in_cr ad t2.
+Proof.
+  solve_incr_preservation
+    onecr_preservation_rel
+    noreacq_preservation_rel.
+Qed.
+
+Corollary incr_preservation_wacq : forall ad t1 t2 ad',
+  in_cr ad t1 ->
+  t1 --[e_wacq ad']--> t2 ->
+  in_cr ad t2.
+Proof.
+  solve_incr_preservation
+    onecr_preservation_wacq
+    noreacq_preservation_wacq.
+Qed.
+
+Corollary incr_preservation_wrel : forall ad t1 t2 ad',
+  ad <> ad' ->
+  in_cr ad t1 ->
+  t1 --[e_wrel ad']--> t2 ->
+  in_cr ad t2.
+Proof.
+  solve_incr_preservation
+    onecr_preservation_wrel
+    noreacq_preservation_wrel.
+Qed.
+
+Corollary incr_preservation_spawn : forall ad m t1 t2 t',
+  valid_term m t1 ->
+  (* --- *)
+  in_cr ad t1 ->
+  t1 --[e_spawn t']--> t2 ->
+  in_cr ad t2.
+Proof.
+  solve_incr_preservation
+    onecr_preservation_spawn
+    noreacq_preservation_spawn.
+Qed.
+
+(* preservation  (nincr) --------------------------------------------------- *)
+
+Local Ltac solve_nincr_preservation L1 L2 :=
+  intros; match goal with H : not_in_cr _ _ |- _ => destruct H end;
+  solve [ left; eauto using nocr_from_value, L1
+        | right; eauto using noreacq_from_value, L2
+        ].
+
+Corollary nincr_preservation_none : forall ad m t1 t2,
+  valid_term m t1 ->
+  (* --- *)
+  not_in_cr ad t1 ->
+  t1 --[e_none]--> t2 ->
+  not_in_cr ad t2.
+Proof.
+  solve_nincr_preservation
+    nocr_preservation_none
+    isw_preservation_none.
+Qed.
+
+Corollary nincr_preservation_alloc : forall ad t1 t2 ad' T',
+  not_in_cr ad t1 ->
+  t1 --[e_alloc ad' T']--> t2 ->
+  not_in_cr ad t2.
+Proof.
+  solve_nincr_preservation
+    nocr_preservation_alloc
+    isw_preservation_alloc.
+Qed.
+
+Corollary nincr_preservation_init : forall ad m t1 t2 ad' t',
+  valid_term m t1 ->
+  (* --- *)
+  not_in_cr ad t1 ->
+  t1 --[e_init ad' t']--> t2 ->
+  not_in_cr ad t2.
+Proof.
+  solve_nincr_preservation
+    nocr_preservation_init
+    isw_preservation_init.
+Qed.
+
+Corollary nincr_preservation_read : forall ad m t1 t2 ad' t',
+  valid_term m t' ->
+  value t'        ->
+  (* --- *)
+  not_in_cr ad t1 ->
+  t1 --[e_read ad' t']--> t2 ->
+  not_in_cr ad t2.
+Proof.
+  solve_nincr_preservation
+    nocr_preservation_read
+    isw_preservation_read.
+Qed.
+
+Corollary nincr_preservation_write : forall ad m t1 t2 ad' t',
+  valid_term m t1 ->
+  (* --- *)
+  not_in_cr ad t1 ->
+  t1 --[e_write ad' t']--> t2 ->
+  not_in_cr ad t2.
+Proof.
+  solve_nincr_preservation
+    nocr_preservation_write
+    isw_preservation_write.
+Qed.
+
+Corollary nincr_preservation_acq : forall ad m t1 t2 ad' t',
+  valid_term m t' ->
+  value t'        ->
+  (* --- *)
+  ad <> ad' ->
+  not_in_cr ad t1 ->
+  t1 --[e_acq ad' t']--> t2 ->
+  not_in_cr ad t2.
+Proof.
+  solve_nincr_preservation
+    nocr_preservation_acq
+    isw_preservation_acq.
+Qed.
+
+Corollary nincr_preservation_rel : forall ad t1 t2 ad',
+  not_in_cr ad t1 ->
+  t1 --[e_rel ad']--> t2 ->
+  not_in_cr ad t2.
+Proof.
+  solve_nincr_preservation
+    nocr_preservation_rel
+    isw_preservation_rel.
+Qed.
+
+Corollary nincr_preservation_wacq : forall ad t1 t2 ad',
+  ad <> ad' ->
+  not_in_cr ad t1 ->
+  t1 --[e_wacq ad']--> t2 ->
+  not_in_cr ad t2.
+Proof.
+  solve_nincr_preservation
+    nocr_preservation_wacq
+    isw_preservation_wacq.
+Qed.
+
+Corollary nincr_preservation_wrel : forall ad t1 t2 ad',
+  ad <> ad' ->
+  not_in_cr ad t1 ->
+  t1 --[e_wrel ad']--> t2 ->
+  not_in_cr ad t2.
+Proof.
+  solve_nincr_preservation
+    nocr_preservation_wrel
+    isw_preservation_wrel.
+Qed.
+
+Corollary nincr_preservation_spawn : forall ad m t1 t2 t',
+  valid_term m t1 ->
+  (* --- *)
+  not_in_cr ad t1 ->
+  t1 --[e_spawn t']--> t2 ->
+  not_in_cr ad t2.
+Proof.
+  solve_nincr_preservation
+    nocr_preservation_spawn
+    isw_preservation_spawn.
+Qed.
+
