SemExt.v
@@ -307,3 +307,56 @@ Proof.
   unfold base. intros. split; eauto using forallmemory_base, forallthreads_base.
 Qed.
 
+(* ------------------------------------------------------------------------- *)
+(* effect inequalities                                                       *)
+(* ------------------------------------------------------------------------- *)
+
+#[export] Hint Extern 8 =>
+  match goal with
+  (* ---------------------------------------------------- *)
+  | _ : ?ad <> ?ad' |- e_init ?ad _ <> e_init ?ad' _ => intros F; invc F
+  | _ : ?ad <> ?ad' |- e_acq  ?ad _ <> e_acq  ?ad' _ => intros F; invc F
+  | _ : ?ad <> ?ad' |- e_rel  ?ad   <> e_rel  ?ad'   => intros F; invc F
+  | _ : ?ad <> ?ad' |- e_wrel ?ad   <> e_wrel ?ad'   => intros F; invc F
+  (* e_init --------------------------------------------- *)
+  | |- e_init _ _ <> e_none      => intros F; invc F
+  | |- e_init _ _ <> e_alloc _ _ => intros F; invc F
+  | |- e_init _ _ <> e_read  _ _ => intros F; invc F
+  | |- e_init _ _ <> e_write _ _ => intros F; invc F
+  | |- e_init _ _ <> e_acq   _ _ => intros F; invc F
+  | |- e_init _ _ <> e_rel   _   => intros F; invc F
+  | |- e_init _ _ <> e_wacq  _   => intros F; invc F
+  | |- e_init _ _ <> e_wrel  _   => intros F; invc F
+  | |- e_init _ _ <> e_spawn _ _ => intros F; invc F
+  (* e_acq ---------------------------------------------- *)
+  | |- e_acq _ _  <> e_none       => intros F; invc F
+  | |- e_acq _ _  <> e_alloc _ _  => intros F; invc F
+  | |- e_acq _ _  <> e_init  _ _  => intros F; invc F
+  | |- e_acq _ _  <> e_read  _ _  => intros F; invc F
+  | |- e_acq _ _  <> e_write _ _  => intros F; invc F
+  | |- e_acq _ _  <> e_rel   _    => intros F; invc F
+  | |- e_acq _ _  <> e_wacq  _    => intros F; invc F
+  | |- e_acq _ _  <> e_wrel  _    => intros F; invc F
+  | |- e_acq _ _  <> e_spawn _ _  => intros F; invc F
+  (* e_rel ---------------------------------------------- *)
+  | |- e_rel _    <> e_none       => intros F; invc F
+  | |- e_rel _    <> e_alloc _ _  => intros F; invc F
+  | |- e_rel _    <> e_init  _ _  => intros F; invc F
+  | |- e_rel _    <> e_read  _ _  => intros F; invc F
+  | |- e_rel _    <> e_write _ _  => intros F; invc F
+  | |- e_rel _    <> e_acq   _ _  => intros F; invc F
+  | |- e_rel _    <> e_wacq  _    => intros F; invc F
+  | |- e_rel _    <> e_wrel  _    => intros F; invc F
+  | |- e_rel _    <> e_spawn _ _  => intros F; invc F
+  (* e_rel ---------------------------------------------- *)
+  | |- e_wrel _   <> e_none       => intros F; invc F
+  | |- e_wrel _   <> e_alloc _ _  => intros F; invc F
+  | |- e_wrel _   <> e_init  _ _  => intros F; invc F
+  | |- e_wrel _   <> e_read  _ _  => intros F; invc F
+  | |- e_wrel _   <> e_write _ _  => intros F; invc F
+  | |- e_wrel _   <> e_acq   _ _  => intros F; invc F
+  | |- e_wrel _   <> e_rel   _    => intros F; invc F
+  | |- e_wrel _   <> e_wacq  _    => intros F; invc F
+  | |- e_wrel _   <> e_spawn _ _  => intros F; invc F
+  end : core.
+
